platform/Xml.v
@@ -1,5 +1,5 @@
 Require Import XmlLang.
-Export XmlLang.
+Export XmlOutput XmlLang.
 
 
 Coercion XmlLang.Cdata : string >-> XmlLang.pat.
@@ -10,15 +10,6 @@ Infix ";;" := XmlLang.Ordered : pat_scope.
 Delimit Scope pat_scope with pat.
 Bind Scope pat_scope with pat.
 
-Coercion XCdata : string >-> xml.
-Notation "$ x" := (XVar x) : out_scope.
-Notation "^ x" := (XColumn x) (at level 0) : out_scope.
-Definition xcons (x : xml) (xs : list xml) : list xml := x :: xs.
-Notation "<*> tag </> x1 , .. , xN </>" := (XTag tag (xcons x1 .. (xcons xN nil) ..))
-  (tag at level 0) : out_scope.
-Delimit Scope out_scope with out.
-Bind Scope out_scope with xml.
-
 Coercion Const : string >-> exp.
 Notation "$ x" := (Input x) : exp_scope.
 Delimit Scope exp_scope with exp.
@@ -28,6 +19,18 @@ Notation "col = e" := ((col, e%exp) :: nil) : condition_scope.
 Infix "&&" := app : condition_scope.
 Delimit Scope condition_scope with condition.
 
+Coercion XCdata : string >-> xml.
+Notation "$ x" := (XVar x) : out_scope.
+Notation "tab # col" := (XColumn tab col) (at level 0) : out_scope.
+Definition xcons (x : xml) (xs : list xml) : list xml := x :: xs.
+Notation "<*> tag </> x1 , .. , xN </>" := (XTag tag (xcons x1 .. (xcons xN nil) ..))
+  (tag at level 0) : out_scope.
+Delimit Scope out_scope with out.
+Notation "'From' tab 'Where' cond 'Write' o" :=
+  (XSelect tab cond%condition o%out)
+  (at level 0, tab at level 0, cond at level 0, o at level 0) : out_scope.
+Bind Scope out_scope with xml.
+
 Definition econs (x : exp) (xs : list exp) : list exp := x :: xs.
 Notation "'Insert' t ( e1 , .. , eN )" := (XmlLang.Insert t (econs e1%exp .. (econs eN%exp nil) ..))
   (at level 0, t at level 0) : action_scope.
@@ -35,9 +38,6 @@ Notation "'Delete' tab 'Where' cond" :=
   (Delete tab cond%condition)
   (at level 0, tab at level 0, cond at level 0) : action_scope.
 Notation "'Write' o" := (Output o%out) (at level 0, o at level 0) : action_scope.
-Notation "'From' tab 'Where' cond 'Write' o" :=
-  (SelectOutput tab cond%condition o%out)
-  (at level 0, tab at level 0, cond at level 0, o at level 0) : action_scope.
 Infix ";;" := Seq : action_scope.
 Delimit Scope action_scope with action.
 Bind Scope action_scope with action.
@@ -47,19 +47,19 @@ Infix ";;" := PSeq : program_scope.
 Delimit Scope program_scope with program.
 Bind Scope program_scope with program.
 
-Ltac wf := split; simpl; intuition (try (congruence || reflexivity || NoDup));
-  match goal with
-      | [ |- Logic.ex _ ] =>
-        match goal with
-          | [ |- context[?e = _] ] => exists e
-        end; unfold ewfs; simpl; intuition;
-        repeat match goal with
-                 | [ |- List.Forall _ _ ] => constructor
-               end; simpl; auto
-    | _ =>
-      repeat match goal with
-               | [ H : List.Exists _ _ |- _ ] => inversion H; clear H; subst
-             end; simpl in *; tauto
-  end; repeat constructor.
-
-Ltac goodSchema := repeat constructor.
+Ltac wf := constructor; try (split || discriminate); simpl;
+  intuition (try (congruence || reflexivity || NoDup));
+    repeat match goal with
+             | [ |- Logic.ex _ ] =>
+               match goal with
+                 | [ |- context[?e = _] ] => exists e
+               end; unfold ewfs; simpl; intuition;
+               repeat match goal with
+                        | [ |- List.Forall _ _ ] => constructor
+                      end; simpl; auto
+             | _ =>
+               repeat match goal with
+                        | [ H : List.Exists _ _ |- _ ] => inversion H; clear H; subst
+                      end; simpl in *; tauto
+             | _ => constructor
+           end.
